<?xml version="1.0" encoding="UTF-8"?>

<rdf:RDF  
    xmlns="https://w3id.org/arm/vocabularies/1.0/typeface/"
    xmlns:dcterms="http://purl.org/dc/terms/"
    xmlns:owl="http://www.w3.org/2002/07/owl#"
    xmlns:rdf="http://www.w3.org/1999/02/22-rdf-syntax-ns#" 
    xmlns:rdfs="http://www.w3.org/2000/01/rdf-schema#"  
    xmlns:skos="http://www.w3.org/2004/02/skos/core#"
    xmlns:vann="http://purl.org/vocab/vann/"
    xmlns:void="http://rdfs.org/ns/void#"
    > 
    
    <skos:ConceptScheme rdf:about="https://w3id.org/arm/vocabularies/1.0/typeface/">
        <dcterms:issued>2018-04-27T00:00:00-04:00</dcterms:issued>
        <dcterms:modified>2021-01-25T00:00:00-04:00</dcterms:modified>
        <skos:prefLabel xml:lang="en">Art and Rare Materials Typeface Vocabulary</skos:prefLabel>
        <skos:definition xml:lang="en">The Art and Rare Materials Typeface Vocabulary is a controlled vocabulary to express the design or “font family” created by a typographer or type designer. Terms represent specific stylistic features to determine the type display of a writing system.</skos:definition>
        <vann:preferredNamespacePrefix>typeface</vann:preferredNamespacePrefix>
    </skos:ConceptScheme> 
    
    <skos:Concept rdf:about="https://w3id.org/arm/vocabularies/1.0/typeface/gothic-antique">
        <rdf:type rdf:resource="http://www.w3.org/2004/02/skos/core#Concept"/>
        <skos:inScheme rdf:resource="https://w3id.org/arm/vocabularies/1.0/typeface/"/>
        <skos:prefLabel xml:lang="en">gothic-antique</skos:prefLabel>
        <skos:definition xml:lang="en">Subgroup of black letter typefaces which are a mix of black letter and roman; rounder and less angular than black letter, and most vertical strokes lack "feet" or ending strokes.</skos:definition>
        <dcterms:issued>2018-04-27T00:00:00-04:00</dcterms:issued>
        <dcterms:modified>2021-01-25T00:00:00-04:00</dcterms:modified>
    </skos:Concept>
    
    <skos:Concept rdf:about="https://w3id.org/arm/vocabularies/1.0/typeface/rotunda">
        <rdf:type rdf:resource="http://www.w3.org/2004/02/skos/core#Concept"/>
        <skos:inScheme rdf:resource="https://w3id.org/arm/vocabularies/1.0/typeface/"/>
        <skos:prefLabel xml:lang="en">rotunda</skos:prefLabel>
        <skos:definition xml:lang="en">Subgroup of black letter typefaces; basically the Southern European black letter.</skos:definition>
        <dcterms:issued>2018-04-27T00:00:00-04:00</dcterms:issued>
        <dcterms:modified>2021-01-25T00:00:00-04:00</dcterms:modified>
    </skos:Concept>
    
    <skos:Concept rdf:about="https://w3id.org/arm/vocabularies/1.0/typeface/textura">
        <rdf:type rdf:resource="http://www.w3.org/2004/02/skos/core#Concept"/>
        <skos:inScheme rdf:resource="https://w3id.org/arm/vocabularies/1.0/typeface/"/>
        <skos:prefLabel xml:lang="en">textura</skos:prefLabel>
        <skos:definition xml:lang="en">Subgroup of black letter typefaces which are squarely drawn and almost completely lacking curves.</skos:definition>
        <dcterms:issued>2018-04-27T00:00:00-04:00</dcterms:issued>
        <dcterms:modified>2021-01-25T00:00:00-04:00</dcterms:modified>
    </skos:Concept>
    
</rdf:RDF>